coq/simple-instance/SCCProof.v
@@ -1,0 +1,57 @@
+Require Import TraceSemantics.
+Require Import Shape.
+Require Import Compiler.
+
+(* _____________________________________ 
+               DEFINITIONS
+   _____________________________________ *)
+
+Reserved Notation "'LOW_NEQ' P '≁L' P'" (at level 40).
+Inductive neq_progL : Target.program -> Target.program -> Prop :=
+  | neqprogL : forall P P',
+    (cprogram_terminates P /\ cprogram_diverges P')
+      \/
+    (cprogram_diverges P /\ cprogram_terminates P')
+      ->
+    (neq_progL P P')
+  where "'LOW_NEQ' P '≁L' P'" := (neq_progL P P').
+
+Reserved Notation "'HIGH_NEQ' P '≁H' P'" (at level 40).
+Inductive neq_progH : Source.program -> Source.program -> Prop :=
+  | neqprog : forall P P',
+    (program_terminates P /\ program_diverges P')
+      \/
+    (program_diverges P /\ program_terminates P')
+      ->
+    (neq_progH P P')
+  where "'HIGH_NEQ' P '≁H' P'" := (neq_progH P P').
+
+
+(* _____________________________________ 
+                 LEMMAS
+   _____________________________________ *)
+
+(* ------- Structured Full Abstraction ------- *)
+
+Theorem structured_full_abstraction :
+  forall s,
+  forall P Q, 
+    (PROGRAM_SHAPE P ∈• s) /\ (PROGRAM_SHAPE Q ∈• s)
+      /\
+    (program_fully_defined s P /\ program_fully_defined s Q)
+    ->
+  forall A,
+    let AP := (context_application A P) in
+    let AQ := (context_application A Q) in 
+    (CONTEXT_SHAPE A ∈∘ s) /\ (context_fully_defined s A)
+    -> HIGH_NEQ AP ≁H AQ
+    -> forall a, (LL_CONTEXT_SHAPE a ∈∘ s) ->
+        LOW_NEQ
+        (LL_context_application a (COMPILE_PROG P↓))
+          ≁L
+        (LL_context_application a (COMPILE_PROG Q↓)).
+Proof.
+Admitted.
+
+
+
